parse32/serialize32 int: do not use loops
This overcomes a Weird unexplained KreMLin error.

A lot of manual code duplication, which could be
avoided by the use of a tactic.

src/lowparse/LowParse.BigEndianImpl.fst
@@ -43,81 +43,120 @@ let be_to_n_body'
   (ensures (fun accu' ->
     u.v accu' == be_to_n (Seq.slice (B32.reveal s) 0 (B32.length s - (U32.v i - 1)))
   ))
-= let sq = G.hide (Seq.slice (B32.reveal s) 0 (B32.length s - U32.v i)) in
+= match u with
+  | UIntType u_v _ u_from_byte _ _ u_add u_mul256 _ ->
+  let sq = G.hide (Seq.slice (B32.reveal s) 0 (B32.length s - U32.v i)) in
   let sq' = G.hide (Seq.slice (B32.reveal s) 0 (B32.length s - (U32.v i - 1))) in
   let b = B32.get s (U32.sub (B32.len s) i) in
   assert (b == Seq.last (G.reveal sq'));
   assert (Seq.slice (G.reveal sq') 0 (Seq.length (G.reveal sq') - 1) == G.reveal sq);
   lemma_be_to_n_is_bounded (G.reveal sq);
   M.pow2_plus (8 `Prims.op_Multiply` Seq.length (G.reveal sq)) 8;
-  assert (u.v accu `Prims.op_Multiply` 256 < pow2 (8 `Prims.op_Multiply` Seq.length (G.reveal sq) + 8));
+  assert (u_v accu `Prims.op_Multiply` 256 < pow2 (8 `Prims.op_Multiply` Seq.length (G.reveal sq) + 8));
   M.pow2_le_compat n (8 `Prims.op_Multiply` Seq.length (G.reveal sq) + 8);
-  assert (u.v accu `Prims.op_Multiply` 256 < pow2 n);
-  let accu256 = u.mul256 accu in
-  let accu' = u.add (u.from_byte b) accu256 in
+  assert (u_v accu `Prims.op_Multiply` 256 < pow2 n);
+  let accu256 = u_mul256 accu in
+  let accu' = u_add (u_from_byte b) accu256 in
   accu'
 
-let be_to_n_inv
-  (t: Type0)
-  (n: nat)
-  (u: uinttype t n)
-  (s: B32.bytes)
-  (continue: bool)
-  (x: U32.t * t)
-: GTot Type0
-= let (i, accu) = x in
-  U32.v i <= B32.length s /\
-  8 `Prims.op_Multiply` B32.length s <= n /\
-  u.v accu == be_to_n (Seq.slice (B32.reveal s) 0 (B32.length s - U32.v i)) /\
-  (continue == false ==> U32.v i == 0)
-
-let be_to_n_measure
-  (t: Type0)
-  (x: U32.t * t)
-: GTot nat
-= let (i, _) = x in
-  U32.v i
-
 inline_for_extraction
-let be_to_n_body
+let be_to_n_1
   (t: Type0)
   (n: nat)
   (u: uinttype t n)
-  (s: B32.bytes)
-  (x: U32.t * t)
-: Pure (bool * (U32.t * t))
-  (requires (be_to_n_inv t n u s true x))
-  (ensures (fun (continue, x') ->
-    be_to_n_inv t n u s continue x' /\
-    (continue == true ==>  be_to_n_measure t x' < be_to_n_measure t x)
-  ))
-= let (i, accu) = x in
-  if i = 0ul
-  then (false, x)
-  else
-    let accu' = be_to_n_body' t n u s i accu in
-    let i' = U32.sub i 1ul in
-    (true, (i', accu'))
-
-module CL = C.Loops
-
-inline_for_extraction
-let be_to_n_impl 
-  (t: Type0)
-  (n: nat)
-  (u: uinttype t n)
-  (s: B32.bytes)
+  (s: B32.lbytes 1)
 : Pure t
-  (requires (8 `Prims.op_Multiply` B32.length s <= n))
-  (ensures (fun y -> u.v y == be_to_n (B32.reveal s)))
-= let (_, res) =
-    CL.total_while
-      (be_to_n_measure t)
-      (be_to_n_inv t n u s)
-      (be_to_n_body t n u s)
-      (B32.len s, u.zero)
+  (requires (
+    Prims.op_Multiply 8 (B32.length s) <= n
+  ))
+  (ensures (fun accu' ->
+    u.v accu' == be_to_n (B32.reveal s)
+  ))
+= match u with
+  | UIntType _ _ _ u_zero _ _ _ _ ->
+  let res =
+    be_to_n_body' t n u s 1ul u_zero
   in
   res
+
+inline_for_extraction
+let be_to_n_2
+  (t: Type0)
+  (n: nat)
+  (u: uinttype t n)
+  (s: B32.lbytes 2)
+: Pure t
+  (requires (
+    Prims.op_Multiply 8 (B32.length s) <= n
+  ))
+  (ensures (fun accu' ->
+    u.v accu' == be_to_n (B32.reveal s)
+  ))
+= match u with
+  | UIntType _ _ _ u_zero _ _ _ _ ->
+  let res2 =
+    be_to_n_body' t n u s 2ul u_zero
+  in
+  let res1 =
+    be_to_n_body' t n u s 1ul res2
+  in
+  res1
+
+inline_for_extraction
+let be_to_n_3
+  (t: Type0)
+  (n: nat)
+  (u: uinttype t n)
+  (s: B32.lbytes 3)
+: Pure t
+  (requires (
+    Prims.op_Multiply 8 (B32.length s) <= n
+  ))
+  (ensures (fun accu' ->
+    u.v accu' == be_to_n (B32.reveal s)
+  ))
+= match u with
+  | UIntType _ _ _ u_zero _ _ _ _ ->
+  let res3 =
+    be_to_n_body' t n u s 3ul u_zero
+  in
+  let res2 =
+    be_to_n_body' t n u s 2ul res3
+  in
+  let res1 =
+    be_to_n_body' t n u s 1ul res2
+  in
+  res1
+
+inline_for_extraction
+let be_to_n_4
+  (t: Type0)
+  (n: nat)
+  (u: uinttype t n)
+  (s: B32.lbytes 4)
+: Pure t
+  (requires (
+    Prims.op_Multiply 8 (B32.length s) <= n
+  ))
+  (ensures (fun accu' ->
+    u.v accu' == be_to_n (B32.reveal s)
+  ))
+= match u with
+  | UIntType _ _ _ u_zero _ _ _ _ ->
+  let res4 =
+    be_to_n_body' t n u s 4ul u_zero
+  in
+  let res3 =
+    be_to_n_body' t n u s 3ul res4
+  in
+  let res2 =
+    be_to_n_body' t n u s 2ul res3
+  in
+  let res1 =
+    be_to_n_body' t n u s 1ul res2
+  in
+  res1
+
 
 inline_for_extraction
 let n_to_be_body'
@@ -144,87 +183,119 @@ let n_to_be_body'
     u.v x' < pow2 (8 `Prims.op_Multiply` U32.v i') /\
     n_to_be (B32.len accu') (u.v x0) == Seq.append (n_to_be i' (u.v x')) (Seq.slice (B32.reveal accu') (U32.v i') (B32.length accu'))
   )))
-= let b = u.to_byte x in
+= match u with
+  | UIntType u_v u_to_byte _ _ _ _ _ u_div256 ->
+  let b = u_to_byte x in
   let i' = U32.sub i 1ul in
   let accu' = B32.set_byte accu i' b in
   M.pow2_plus 8 (8 `Prims.op_Multiply` U32.v i');
-  let x' = G.hide (u.div256 x) in
-  assert (u.v (G.reveal x') < pow2 (8 `Prims.op_Multiply` U32.v i'));
-  assert (n_to_be i (u.v x) == Seq.append (n_to_be i' (u.v (G.reveal x'))) (Seq.create 1 b));
+  let x' = G.hide (u_div256 x) in
+  assert (u_v (G.reveal x') < pow2 (8 `Prims.op_Multiply` U32.v i'));
+  assert (n_to_be i (u_v x) == Seq.append (n_to_be i' (u_v (G.reveal x'))) (Seq.create 1 b));
   assert (Seq.slice (B32.reveal accu') (U32.v i) (B32.length accu') == Seq.slice (B32.reveal accu) (U32.v i) (B32.length accu));
   assert (Seq.slice (B32.reveal accu') (U32.v i') (B32.length accu') `Seq.equal` Seq.append (Seq.create 1 b) (Seq.slice (B32.reveal accu') (U32.v i) (B32.length accu')));
-  Seq.append_assoc (n_to_be i' (u.v (G.reveal x'))) (Seq.create 1 b) (Seq.slice (B32.reveal accu') (U32.v i) (B32.length accu'));
+  Seq.append_assoc (n_to_be i' (u_v (G.reveal x'))) (Seq.create 1 b) (Seq.slice (B32.reveal accu') (U32.v i) (B32.length accu'));
   accu'
 
-let n_to_be_inv
-  (t: Type0)
-  (n: nat)
-  (u: uinttype t n)
-  (len: U32.t)
-  (x0: t)
-  (continue: bool)
-  (y: U32.t * t * B32.bytes)
-: GTot Type0
-= let (i, x, accu) = y in
-    U32.v len == B32.length accu /\
-    8 `Prims.op_Multiply` B32.length accu <= n /\
-    U32.v i <= B32.length accu /\
-    u.v x0 < pow2 (8 `Prims.op_Multiply` B32.length accu) /\
-    u.v x < pow2 (8 `Prims.op_Multiply` U32.v i) /\
-    n_to_be (B32.len accu) (u.v x0) == Seq.append (n_to_be i (u.v x)) (Seq.slice (B32.reveal accu) (U32.v i) (B32.length accu)) /\
-    (continue == false ==> U32.v i == 0)
-
-let n_to_be_measure
-  (t: Type0)
-  (y: U32.t * t * B32.bytes)
-: GTot nat
-= let (i, _, _) = y in
-  U32.v i
-
 inline_for_extraction
-let n_to_be_body
+let n_to_be_1
   (t: Type0)
   (n: nat)
   (u: uinttype t n)
-  (len: U32.t)
   (x0: t)
-  (y: U32.t * t * B32.bytes)
-: Pure (bool * (U32.t * t * B32.bytes))
-  (requires (n_to_be_inv t n u len x0 true y))
-  (ensures (fun (continue, y') ->
-    n_to_be_inv t n u len x0 continue y' /\
-    (continue == true ==> n_to_be_measure t y' < n_to_be_measure t y)
+: Pure B32.bytes
+  (requires (
+    8 `Prims.op_Multiply` 1 <= n /\
+    u.v x0 < pow2 (8 `Prims.op_Multiply` 1)
   ))
-= let (i, x, accu) = y in
-  if i = 0ul
-  then (false, y)
-  else
-    let accu' = n_to_be_body' t n u x0 i x accu in
-    let x' = u.div256 x in
-    let i' = U32.sub i 1ul in
-    (true, (i', x', accu'))
+  (ensures (fun accu' ->
+    B32.length accu' == 1 /\
+    n_to_be 1ul (u.v x0) == B32.reveal accu'
+  ))
+= let accu = B32.create 1ul 42uy in
+  Seq.append_empty_r (n_to_be 1ul (u.v x0));
+  let res = n_to_be_body' t n u x0 1ul x0 accu in
+  Seq.append_empty_l (B32.reveal res);
+  res
 
 inline_for_extraction
-let n_to_be_impl
+let n_to_be_2
   (t: Type0)
   (n: nat)
   (u: uinttype t n)
-  (len: U32.t)
   (x0: t)
-  (z: unit {
-    u.v x0 < pow2 (8 `Prims.op_Multiply` U32.v len) /\
-    8 `Prims.op_Multiply` U32.v len <= n
-  } )
-: Tot (y: B32.bytes { B32.reveal y == n_to_be len (u.v x0) } )
-= let buf = B32.create len 42uy in
-  Seq.append_empty_r (n_to_be len (u.v x0));
-  let (_, _, res) =
-    CL.total_while
-      (n_to_be_measure t)
-      (n_to_be_inv t n u len x0)
-      (n_to_be_body t n u len x0)
-      (len, x0, buf)
-  in
+: Pure B32.bytes
+  (requires (
+    8 `Prims.op_Multiply` 2 <= n /\
+    u.v x0 < pow2 (8 `Prims.op_Multiply` 2)
+  ))
+  (ensures (fun accu' ->
+    B32.length accu' == 2 /\
+    n_to_be 2ul (u.v x0) == B32.reveal accu'
+  ))
+= match u with
+  | UIntType u_v u_to_byte _ _ _ _ _ u_div256 ->
+  let accu = B32.create 2ul 42uy in
+  Seq.append_empty_r (n_to_be 2ul (u.v x0));
+  let accu1 = n_to_be_body' t n u x0 2ul x0 accu in
+  let x1 = u_div256 x0 in
+  let res = n_to_be_body' t n u x0 1ul x1 accu1 in
+  Seq.append_empty_l (B32.reveal res);
+  res
+
+inline_for_extraction
+let n_to_be_3
+  (t: Type0)
+  (n: nat)
+  (u: uinttype t n)
+  (x0: t)
+: Pure B32.bytes
+  (requires (
+    8 `Prims.op_Multiply` 3 <= n /\
+    u.v x0 < pow2 (8 `Prims.op_Multiply` 3)
+  ))
+  (ensures (fun accu' ->
+    B32.length accu' == 3 /\
+    n_to_be 3ul (u.v x0) == B32.reveal accu'
+  ))
+= match u with
+  | UIntType u_v u_to_byte _ _ _ _ _ u_div256 ->
+  let accu = B32.create 3ul 42uy in
+  Seq.append_empty_r (n_to_be 3ul (u.v x0));
+  let accu2 = n_to_be_body' t n u x0 3ul x0 accu in
+  let x2 = u_div256 x0 in
+  let accu1 = n_to_be_body' t n u x0 2ul x2 accu2 in
+  let x1 = u_div256 x2 in
+  let res = n_to_be_body' t n u x0 1ul x1 accu1 in
+  Seq.append_empty_l (B32.reveal res);
+  res
+
+inline_for_extraction
+let n_to_be_4
+  (t: Type0)
+  (n: nat)
+  (u: uinttype t n)
+  (x0: t)
+: Pure B32.bytes
+  (requires (
+    8 `Prims.op_Multiply` 4 <= n /\
+    u.v x0 < pow2 (8 `Prims.op_Multiply` 4)
+  ))
+  (ensures (fun accu' ->
+    B32.length accu' == 4 /\
+    n_to_be 4ul (u.v x0) == B32.reveal accu'
+  ))
+= match u with
+  | UIntType u_v u_to_byte _ _ _ _ _ u_div256 ->
+  let accu = B32.create 4ul 42uy in
+  Seq.append_empty_r (n_to_be 4ul (u.v x0));
+  let accu3 = n_to_be_body' t n u x0 4ul x0 accu in
+  let x3 = u_div256 x0 in
+  let accu2 = n_to_be_body' t n u x0 3ul x3 accu3 in
+  let x2 = u_div256 x3 in
+  let accu1 = n_to_be_body' t n u x0 2ul x2 accu2 in
+  let x1 = u_div256 x2 in
+  let res = n_to_be_body' t n u x0 1ul x1 accu1 in
   Seq.append_empty_l (B32.reveal res);
   res
 
@@ -234,7 +305,7 @@ module U32 = FStar.UInt32
 module Cast = FStar.Int.Cast
 
 inline_for_extraction
-let u8 : uinttype U8.t 8 =
+let u8 () : uinttype U8.t 8 =
   UIntType
     (fun x -> U8.v x)
     (fun x -> x)
@@ -246,7 +317,7 @@ let u8 : uinttype U8.t 8 =
     (fun x -> 0uy)
 
 inline_for_extraction
-let u16 : uinttype U16.t 16 =
+let u16 () : uinttype U16.t 16 =
   UIntType
     (fun x -> U16.v x)
     (fun x -> Cast.uint16_to_uint8 x)
@@ -258,7 +329,7 @@ let u16 : uinttype U16.t 16 =
     (fun x -> U16.div x 256us)
 
 inline_for_extraction
-let u32 : uinttype U32.t 32 =
+let u32 () : uinttype U32.t 32 =
   UIntType
     (fun x -> U32.v x)
     (fun x -> Cast.uint32_to_uint8 x)
